ulib/FStar.Math.Fermat.fsti
@@ -2,7 +2,7 @@ module FStar.Math.Fermat
 
 open FStar.Mul
 open FStar.Math.Euclid
-    
+
 /// Fermat's Little Theorem (and Binomial Theorem)
 ///
 /// Proven by induction from the Freshman's dream identity
@@ -28,12 +28,10 @@ let rec pow (a:int) (k:nat) : int =
   if k = 0 then 1
   else a * pow a (k - 1)
 
-val fermat (p:pos{1 < p /\ is_prime p}) (a:int) : Lemma 
-  (pow a p % p == a % p)
+val fermat (p:int{is_prime p}) (a:int) : Lemma (pow a p % p == a % p)
 
-val mod_mult_congr (p:pos{1 < p /\ is_prime p}) (a b c:int) : Lemma
+val mod_mult_congr (p:int{is_prime p}) (a b c:int) : Lemma
   (requires (a * c) % p = (b * c) % p /\ c % p <> 0)
   (ensures  a % p = b % p)
 
-val fermat_alt (p:pos{1 < p /\ is_prime p}) (a:int{a % p <> 0}) : Lemma 
-  (pow a (p - 1) % p == 1)
+val fermat_alt (p:int{is_prime p}) (a:int{a % p <> 0}) : Lemma (pow a (p - 1) % p == 1)
